FOL_Compactness/Skolem_Normal_Form.thy
@@ -1,0 +1,35 @@
+(* Title:        Part of the proof of compactness of first-order logic following Harrison's one in
+ *               HOL-Light
+ * Author:       Sophie Tourret <sophie.tourret at inria.fr>, 2023 *)
+
+theory Skolem_Normal_Form
+imports
+  Prenex_Normal_Form
+begin
+
+lemma holds_exists:
+  assumes \<open>is_interpretation (functions_term t) preds (I :: (nat, nat) term intrp)\<close> and
+    \<open>is_valuation I \<beta>\<close> and 
+    \<open>I, \<beta> \<Turnstile> (\<phi> \<cdot>\<^sub>f\<^sub>m (subst x t))\<close>
+  shows \<open>I, \<beta> \<Turnstile> (\<^bold>\<exists>x\<^bold>. \<phi>)\<close>
+proof -
+  have \<open>(\<lambda>v. \<lbrakk>subst x t v\<rbrakk>\<^bsup>I,\<beta>\<^esup>) = \<beta>(x := \<lbrakk>t\<rbrakk>\<^bsup>I,\<beta>\<^esup>)\<close>
+  proof -
+    have "\<forall>n. \<lbrakk>subst x t n\<rbrakk>\<^bsup>I,\<beta>\<^esup> = (\<beta>(x := \<lbrakk>t\<rbrakk>\<^bsup>I,\<beta>\<^esup>)) n"
+      by (simp add: subst_def)
+    then show ?thesis
+      by blast
+  qed
+  moreover have \<open>\<lbrakk>t\<rbrakk>\<^bsup>I,\<beta>\<^esup> \<in> dom I\<close>
+    using interpretation_termval[OF assms(1) assms(2)] .
+  ultimately have \<open>\<exists>a \<in> dom I. I, \<beta>(x := a) \<Turnstile> \<phi>\<close>
+    using assms(3) swap_subst_eval[of I \<beta> \<phi> "subst x t"] by auto
+  then show ?thesis
+    using holds_exists by blast
+qed
+
+find_theorems \<open>_ \<in> dom _ \<close> dom
+
+find_theorems \<open>\<lbrakk>_\<rbrakk>\<^bsup>_,_\<^esup>\<close>
+
+end
